more wip towards the top-level lemma ... getting there

vale/code/arch/x64/interop/Vale.AsLowStar.LowStarSig.fst
@@ -57,15 +57,12 @@ let hsprop = HS.mem -> VS.state -> prop
 [@reduce]
 let to_low_pre
     (pre:VSig.vale_pre_tl [])
-    (args_disjointness:prop)
-    (args_liveness:hprop)
+    (args:list arg)
     (arg_pre_hyp:sprop)
     (mem_correspondence:hsprop)
     (num_stack_slots:nat)
-    (hs_mem:HS.mem)
+    (hs_mem:mem_roots args)
   : prop =
-  args_disjointness /\
-  args_liveness hs_mem /\
   (forall (s0:V.va_state)
      (sb:IX64.stack_buffer).
     s0.VS.ok /\
@@ -77,17 +74,16 @@ let to_low_pre
 [@reduce]
 let to_low_post
     (post:VSig.vale_post_tl [])
+    (args:list arg)
     (args_fp:B.loc)
-    (args_liveness:hprop)
     (mem_correspondence: hsprop)
-    (hs_mem0:HS.mem)
+    (hs_mem0:mem_roots args)
     (_:unit)
-    (hs_mem1:HS.mem)
+    (hs_mem1:mem_roots args)
   : prop =
   let open V in
   // REVIEW: it would be more flexible to let low_assumptions/post take care of modifies:
   B.modifies args_fp hs_mem0 hs_mem0 /\
-  args_liveness hs_mem1 /\
   (exists
     (s0:va_state)
     (sb:IX64.stack_buffer)
@@ -208,9 +204,11 @@ let vale_pre_hyp (args:IX64.arity_ok arg) : sprop =
       register_args (List.length args) args s0 /\
       taint_hyp args s0
 
+
 [@reduce]
-let rec as_lowstar_sig_tl
+let rec lowstar_lemma_typ
           (#dom:list td)
+          (code:V.va_code)
           (args:list arg{List.length args + List.length dom < IX64.max_arity})
           (num_stack_slots:nat)
           (pre:VSig.vale_pre_tl dom)
@@ -219,32 +217,22 @@ let rec as_lowstar_sig_tl
     let open FStar.HyperStack.ST in
     match dom with
     | [] ->
-      let liveness h = all_live h args in
       let mem_corr = mem_correspondence args in
-      unit ->
-      Stack unit
-        (requires (to_low_pre pre (disjoint_or_eq args) liveness (vale_pre_hyp args) mem_corr num_stack_slots))
-        (ensures (to_low_post post (mk_modifies_loc args) liveness mem_corr))
+      h0:mem_roots args ->
+      predict:IX64.prediction (coerce code) args h0 ->
+      ret:IX64.as_lowstar_sig_ret args ->
+      h1:mem_roots args ->
+      Lemma
+        (requires (to_low_pre pre args (vale_pre_hyp args) mem_corr num_stack_slots h0 /\
+                   IX64.as_lowstar_sig_post (coerce code) args h0 predict ret h1))
+        (ensures (to_low_post post args (mk_modifies_loc args) mem_corr h0 () h1))
 
     | hd::tl ->
       x:td_as_type hd ->
-      as_lowstar_sig_tl
+      lowstar_lemma_typ
         #tl
+        code
         ((| hd, x |)::args)
         num_stack_slots
         (elim_1 pre x)
         (elim_1 post x)
-
-[@reduce]
-let as_lowstar_sig
-       (c:V.va_code)
-       (dom:IX64.arity_ok td)
-       (num_stack_slots:nat)
-       (pre: VSig.vale_pre dom)
-       (post: VSig.vale_post dom) =
-    as_lowstar_sig_tl
-      #dom
-      []
-      num_stack_slots
-      (pre c)
-      (post c)
