vale/code/arch/x64/interop/Vale.AsLowStar.Wrapper.fst
@@ -37,7 +37,7 @@ module LSig = Vale.AsLowStar.LowStarSig
 module SL = X64.Vale.StateLemmas
 // module BS = X64.Bytes_Semantics_s
 // module MS = X64.Memory_Sems
-
+module VL = X64.Vale.Lemmas
 
 [@reduce]
 let create_initial_vale_state
@@ -69,75 +69,210 @@ let core_create_lemma
     (h0:HS.mem)
     (stack:b8{mem_roots_p h0 (IX64.arg_of_b8 stack::args)})
   : Lemma
-      (ensures (fst (IX64.create_initial_trusted_state args h0 stack) ==
-                SL.state_to_S (create_initial_vale_state args h0 stack)))
+      (ensures (let va_s = create_initial_vale_state args h0 stack in
+                fst (IX64.create_initial_trusted_state args h0 stack) == SL.state_to_S va_s /\
+                LSig.mem_correspondence args h0 va_s /\
+                LSig.mk_vale_disjointness args /\
+                LSig.mk_readable args va_s /\
+                LSig.vale_pre_hyp args va_s))
   = admit() //needs the definition of SL.state_to_S; not sure why its hidden in StateLemma
+
+let frame_mem_correspondence
+       (args:list arg)
+       (h0:mem_roots args)
+       (h1:mem_roots args)
+       (va_s:V.va_state)
+ : Lemma
+     (requires
+       LSig.mem_correspondence args h1 va_s /\
+       B.modifies B.loc_none h0 h1)
+     (ensures
+       LSig.mem_correspondence args h0 va_s)
+ = admit()
+
+
+
 module ST = FStar.HyperStack.ST
+assume
+val fuel_eq : squash (V.va_fuel == nat)
 
-let code_equiv : squash (V.va_code == TS.tainted_code) = admit()
 
-let rec wrap_aux
-         (code:V.va_code)
-         (dom:list td)
-         (args:list arg{List.length args + List.length dom < IX64.max_arity})
-         (num_stack_slots:nat)
-         (pre:VSig.vale_pre_tl dom)
-         (post:VSig.vale_post_tl dom)
-         (v:VSig.vale_sig_tl args code pre post)
-    : LSig.as_lowstar_sig_tl args num_stack_slots pre post
-    = match dom with
-      | [] ->
-        let code : TS.tainted_code = coerce code in
-        let f : LSig.as_lowstar_sig_tl #[] args num_stack_slots pre post =
-          fun () ->
-            let h0 = ST.get () in
-            let f_predict
-                (s0:TS.traceState)
-                (push_h0:mem_roots args)
-                (alloc_push_h0:mem_roots args)
-                (b:IX64.stack_buffer{mem_roots_p alloc_push_h0 (IX64.arg_of_b8 b::args)})
-              : Ghost (nat & ME.mem)
-                  (requires IX64.prediction_pre code args h0 s0 push_h0 alloc_push_h0 b)
-                  (ensures IX64.prediction_post code args h0 s0 push_h0 alloc_push_h0 b)
-                = admit()
-                // let va_s0 = elim_down_nil acc v_down alloc_push_h0 b in
-                // let va_s1, fuel = elim_vale_sig_nil pre post v va_s0 (to_b8 b) in
-                // (fuel, va_s1.mem)
-            in
-            let predict : IX64.prediction code args h0 = f_predict in
-            let IX64.As_lowstar_sig_ret push_h0 alloc_push_h0 b fuel final_mem =
-              IX64.wrap code args h0 predict
-            in
-            admit()
-            // let h1 = get () in
-            // assert (
-            //   let initial_state = elim_down_nil acc v_down alloc_push_h0 b in
-            //   let (final, fuel) = elim_vale_sig_nil pre post v initial_state b in
-            //   eval_code code initial_state fuel final
-            // );
-            // ()
-        in
-        f <: LSig.as_lowstar_sig_tl #[] args num_stack_slots pre post
-      | hd::tl ->
-        let f (x:td_as_type hd) =
-          wrap_aux
-              code
-              tl
-              ((|hd,x|)::args)
+let eval_code_ts (c:TS.tainted_code)
+                 (s0:TS.traceState)
+                 (f0:nat)
+                 (s1:TS.traceState) : Type0 =
+  VL.state_eq_opt (TS.taint_eval_code c f0 s0) (Some s1)
+
+let eval_code_rel (c:TS.tainted_code)
+                  (va_s0 va_s1:_) (f:V.va_fuel)
+  : Lemma
+     (requires (V.eval_code c va_s0 f va_s1))
+     (ensures (eval_code_ts c (SL.state_to_S va_s0) (coerce f) (SL.state_to_S va_s1)))
+  = admit()
+
+assume
+val increase_fuel (c:TS.tainted_code)
+                  (s0:TS.traceState)
+                  (f0:nat)
+                  (sN:TS.traceState)
+                  (fN:nat) : Lemma
+  (requires eval_code_ts c s0 f0 sN /\ f0 <= fN)
+  (ensures eval_code_ts c s0 fN sN)
+
+let fuel_irrelevance (c:TS.tainted_code)
+                     (s0:TS.traceState)
+                     (f1:nat)
+                     (s1:TS.traceState)
+                     (f2:nat)
+                     (s2:TS.traceState)
+  : Lemma
+  (requires eval_code_ts c s0 f1 s1 /\
+            eval_code_ts c s0 f2 s2)
+  (ensures  VL.state_eq_opt (Some s1) (Some s2))
+  = if f1 <= f2 then increase_fuel c s0 f1 s1 f2
+    else increase_fuel c s0 f2 s2 f1
+
+////////////////////////////////////////////////////////////////////////////////
+
+let lowstar_lemma_base
+          (code:V.va_code)
+          (args:IX64.arity_ok arg)
+          (num_stack_slots:nat)
+          (pre:VSig.vale_pre_tl [])
+          (post:VSig.vale_post_tl [])
+          (v:VSig.vale_sig_tl args (coerce code) pre post)
+          (h0:mem_roots args)
+          (predict:IX64.prediction (coerce code) args h0)
+          (ret:IX64.as_lowstar_sig_ret args)
+          (h1:mem_roots args)
+  : Lemma
+      (requires (LSig.(to_low_pre pre args (vale_pre_hyp args) (mem_correspondence args) num_stack_slots h0 /\
+                 IX64.as_lowstar_sig_post (coerce code) args h0 predict ret h1)))
+      (ensures LSig.(to_low_post post args (mk_modifies_loc args) (mem_correspondence args) h0 () h1))
+  = let open LSig in
+    let open IX64 in
+    let As_lowstar_sig_ret push_h0 alloc_push_h0 stack_buf fuel final_mem = ret in
+    let s0 = fst (create_initial_trusted_state args alloc_push_h0 stack_buf) in
+    let Some s1 = TS.taint_eval_code (coerce code) fuel s0 in
+    let va_s0 = create_initial_vale_state args alloc_push_h0 stack_buf in
+    core_create_lemma args alloc_push_h0 stack_buf;
+    assert (SL.state_to_S va_s0 == s0);
+    B.fresh_frame_modifies h0 push_h0;
+    assert (B.modifies B.loc_none h0 alloc_push_h0);
+    assert (mem_correspondence args alloc_push_h0 va_s0);
+    frame_mem_correspondence args h0 alloc_push_h0 va_s0;
+    assert (mem_correspondence args h0 va_s0);
+    assert (va_s0.VS.ok);
+    assert (vale_pre_hyp args va_s0);
+    assume (V.valid_stack_slots
+              va_s0.VS.mem
+              (VS.eval_reg MS.Rsp va_s0)
+              (as_vale_buffer stack_buf)
               num_stack_slots
-              (elim_1 pre x)
-              (elim_1 post x)
-              (VSig.elim_vale_sig_cons hd tl args pre post v x)
-        in
-        f
+              va_s0.VS.memTaint);
+    assert (elim_nil pre va_s0 stack_buf);
+    let va_s1, f = VSig.elim_vale_sig_nil v va_s0 stack_buf in
+    assert (V.eval_code (coerce code) va_s0 f va_s1);
+    eval_code_rel (coerce code) va_s0 va_s1 f;
+    let Some s1' = TS.taint_eval_code (coerce code) (coerce f) s0 in
+    fuel_irrelevance (coerce code) s0 fuel s1 (coerce f) s1';
+    assert (VL.state_eq_opt (Some (SL.state_to_S va_s1)) (Some s1));
+    assert (VSig.vale_calling_conventions va_s0 va_s1);
+    assert (elim_nil post va_s0 stack_buf va_s1 f);
+    assert (ME.modifies (VSig.fp_of_args args) va_s0.VS.mem va_s1.VS.mem);
+    let h1_pre_pop // : mem_roots args
+      = Interop.Adapters.hs_of_mem final_mem in
+    assume (mem_correspondence args h1_pre_pop va_s1);
+//    let h1_pre = IM.down_mem
+    assert (HS.poppable h1_pre_pop);
+    assert (h1 == HS.pop h1_pre_pop);
+    assume (mem_correspondence args h1 va_s1)
+
+// let rec lowstar_lemma
+//           (dom:list td)
+//           (code:V.va_code)
+//           (args:list arg{List.length args + List.length dom < IX64.max_arity})
+//           (num_stack_slots:nat)
+//           (pre:VSig.vale_pre_tl dom)
+//           (post:VSig.vale_post_tl dom)
+//           (v:VSig.vale_sig_tl args (coerce code) pre post)
+//     : lowstar_lemma_typ code args num_stack_slots pre post
+//     = match dom with
+//       | [] ->
+//         lowstar_lemma_base code args num_stack_slots pre post v
+//       | hd::tl ->
+//         fun (x:td_as_type hd) ->
+//           lowstar_lemma
+//             tl
+//             code
+//             ((| hd, x |) :: args)
+//             num_stack_slots
+//             (elim_1 pre x)
+//             (elim_1 post x)
+//             (VSig.elim_vale_sig_cons hd tl args pre post v x)
+
+// let rec wrap_aux
+//          (code:V.va_code)
+//          (dom:list td)
+//          (args:list arg{List.length args + List.length dom < IX64.max_arity})
+//          (num_stack_slots:nat)
+//          (pre:VSig.vale_pre_tl dom)
+//          (post:VSig.vale_post_tl dom)
+//          (v:VSig.vale_sig_tl args code pre post)
+//     : LSig.as_lowstar_sig_tl args num_stack_slots pre post
+//     = match dom with
+//       | [] ->
+//         let code : TS.tainted_code = coerce code in
+//         let f : LSig.as_lowstar_sig_tl #[] args num_stack_slots pre post =
+//           fun () ->
+//             let h0 = ST.get () in
+//             let f_predict
+//                 (s0:TS.traceState)
+//                 (push_h0:mem_roots args)
+//                 (alloc_push_h0:mem_roots args)
+//                 (b:IX64.stack_buffer{mem_roots_p alloc_push_h0 (IX64.arg_of_b8 b::args)})
+//               : Ghost (nat & ME.mem)
+//                   (requires IX64.prediction_pre code args h0 s0 push_h0 alloc_push_h0 b)
+//                   (ensures IX64.prediction_post code args h0 s0 push_h0 alloc_push_h0 b)
+//                 = admit()
+//                 // let va_s0 = elim_down_nil acc v_down alloc_push_h0 b in
+//                 // let va_s1, fuel = elim_vale_sig_nil pre post v va_s0 (to_b8 b) in
+//                 // (fuel, va_s1.mem)
+//             in
+//             let predict : IX64.prediction code args h0 = f_predict in
+//             let IX64.As_lowstar_sig_ret push_h0 alloc_push_h0 b fuel final_mem =
+//               IX64.wrap code args h0 predict
+//             in
+//             admit()
+//             // let h1 = get () in
+//             // assert (
+//             //   let initial_state = elim_down_nil acc v_down alloc_push_h0 b in
+//             //   let (final, fuel) = elim_vale_sig_nil pre post v initial_state b in
+//             //   eval_code code initial_state fuel final
+//             // );
+//             // ()
+//         in
+//         f <: LSig.as_lowstar_sig_tl #[] args num_stack_slots pre post
+//       | hd::tl ->
+//         let f (x:td_as_type hd) =
+//           wrap_aux
+//               code
+//               tl
+//               ((|hd,x|)::args)
+//               num_stack_slots
+//               (elim_1 pre x)
+//               (elim_1 post x)
+//               (VSig.elim_vale_sig_cons hd tl args pre post v x)
+//         in
+//         f
 
 
-let wrap
-    (code:V.va_code)
-    (dom:IX64.arity_ok td)
-    (num_stack_slots:nat)
-    (pre:VSig.vale_pre dom)
-    (post:VSig.vale_post dom)
-    (v:VSig.vale_sig pre post)
-  : LSig.as_lowstar_sig code dom num_stack_slots pre post
-  = wrap_aux code dom [] num_stack_slots (pre code) (post code) (v code IA.win)
+// let wrap
+//     (code:V.va_code)
+//     (dom:IX64.arity_ok td)
+//     (num_stack_slots:nat)
+//     (pre:VSig.vale_pre dom)
+//     (post:VSig.vale_post dom)
+//     (v:VSig.vale_sig pre post)
+//   : LSig.as_lowstar_sig code dom num_stack_slots pre post
+//   = wrap_aux code dom [] num_stack_slots (pre code) (post code) (v code IA.win)
