vale/specs/interop/Interop.X64.fst
@@ -13,30 +13,33 @@ let wrap c args h0 predict =
   let h0' = ST.get () in
   assert (mem_roots_p h0' args);
   ST.push_frame ();
-  let h1 = ST.get () in
-  B.fresh_frame_modifies h0' h1;
-  mem_roots_p_modifies_none args h0' h1;
+  let push_h0 = ST.get () in
+  B.fresh_frame_modifies h0' push_h0;
+  mem_roots_p_modifies_none args h0' push_h0;
   let stack_b : lowstar_buffer ME.(TBase TUInt8) = B.alloca (UInt8.uint_to_t 0) (UInt32.uint_to_t 24) in
-  let h2 = ST.get () in
-  assert (HS.fresh_frame h0 h1);
-  mem_roots_p_modifies_none args h1 h2;
-  assert (mem_roots_p h2 args);
+  let alloc_push_h0 = ST.get () in
+  assert (HS.fresh_frame h0 push_h0);
+  mem_roots_p_modifies_none args push_h0 alloc_push_h0;
+  assert (mem_roots_p alloc_push_h0 args);
   let sarg = arg_of_lb stack_b in
-  all_live_cons sarg args h2;
+  all_live_cons sarg args alloc_push_h0;
   disjoint_or_eq_cons sarg args;
-  disjoint_or_eq_fresh stack_b args h1;
-  assert (mem_roots_p h2 (sarg::args));
+  disjoint_or_eq_fresh stack_b args push_h0;
+  assert (mem_roots_p alloc_push_h0 (sarg::args));
   let (fuel, final_mem) =
     IA.st_put
-      (fun h0' -> h0' == h2)
+      (fun h0' -> h0' == alloc_push_h0)
       (fun h0' ->
         let va_s0, mem_s0 =
           create_initial_trusted_state args h0' stack_b in
-        let (fuel, final_mem) = predict va_s0 h1 h2 stack_b in
+        let (fuel, final_mem) = predict va_s0 push_h0 alloc_push_h0 stack_b in
         assert (B.frameOf stack_b = HS.get_tip h0');
         assert (B.live h0' stack_b);
         let Some va_s1 = TS.taint_eval_code c fuel va_s0 in
+        let final_hs = Adapters.hs_of_mem final_mem in
+//        assume (ST.equal_domains alloc_push_h0 final_hs);
         ((fuel, final_mem), Adapters.hs_of_mem final_mem)
-      ) in //conveniently, st_put assumes that the shape of the stack did not change
+      ) in //too conveniently, st_put assumes that the shape of the stack did not change; TODO: FIX THAT!
   ST.pop_frame ();
-  As_lowstar_sig_ret h1 h2 stack_b fuel final_mem
+  assert (ST.equal_domains alloc_push_h0 (Adapters.hs_of_mem final_mem));
+  As_lowstar_sig_ret push_h0 alloc_push_h0 stack_b fuel final_mem
